Structure the proof of global simulation.

backend/RTLGlobalSim.v
@@ -9,7 +9,6 @@ Require Import Events.
 Require Import Memory.
 Require Import Globalenvs.
 Require Import Smallstep.
-Require Import IndexedStep.
 Require Import Op.
 Require Import Registers.
 Require Import RTL.
@@ -38,38 +37,50 @@ Hypothesis
 
 Variable (mrel_init:mrelT). (* TODO *)
 
-Inductive match_stackframes: forall (mrel:mrelT) (cs_src cs_tgt:list stackframe), Prop :=
+Inductive match_stackframes: forall (height:nat) (mrel:mrelT) (cs_src cs_tgt:list stackframe), Prop :=
 | match_stackframes_nil:
-    match_stackframes mrel_init nil nil
+    match_stackframes 0 mrel_init nil nil
 | match_stackframes_cons
-    ps_src ps_tgt s_src s_tgt
-    pmrel mrel
-    (Hp: match_stackframes pmrel ps_src ps_tgt)
-    (Hmrel_le: mrelT_ops.(le) pmrel mrel)
+    height ps_src ps_tgt s_src s_tgt
+    emrel mrel
+    (Hp: match_stackframes height emrel ps_src ps_tgt)
+    (Hmrel_le: mrelT_ops.(le) emrel mrel)
     (Hreturn:
-       forall rmrel st_src st_tgt mem_src mem_tgt vres_src vres_tgt
+       forall rmrel ri st_src st_tgt mem_src mem_tgt vres_src vres_tgt
               (Hvres: mrelT_ops.(sem_value) rmrel vres_src vres_tgt)
-              (Hst2_src: st_src = Returnstate s_src vres_src mem_src)
-              (Hst2_tgt: st_tgt = Returnstate s_tgt vres_tgt mem_tgt)
+              (Hst_src: st_src = Returnstate s_src vres_src mem_src)
+              (Hst_tgt: st_tgt = Returnstate s_tgt vres_tgt mem_tgt)
               (Hsound_src: sound_state_ext prog_src st_src)
               (Hsound_tgt: sound_state_ext prog_tgt st_tgt)
-              (Hmrel2_le: mrelT_ops.(le_public) mrel rmrel)
-              (Hst2_mem: mrelT_ops.(sem) rmrel mem_src mem_tgt),
-       exists ri,
-         state_lsim mrelT_ops prog_src prog_tgt ps_src ps_tgt mrel rmrel ri st_src st_tgt):
-    match_stackframes mrel s_src s_tgt
+              (Hrmrel_le: mrelT_ops.(le_public) mrel rmrel)
+              (Hst_mem: mrelT_ops.(sem) rmrel mem_src mem_tgt),
+         state_lsim mrelT_ops prog_src prog_tgt ps_src ps_tgt emrel rmrel ri st_src st_tgt):
+    match_stackframes (S height) mrel s_src s_tgt
 .
 
 Inductive match_states (i:WF.t) (st_src st_tgt:state): Prop :=
 | match_states_intro
-    ps_src ps_tgt
-    pmrel mrel
-    (Hp: match_stackframes pmrel ps_src ps_tgt)
-    (Hmrel_le: mrelT_ops.(le) pmrel mrel)
-    (Hsound_src: sound_state_ext prog_src st_src)
-    (Hsound_tgt: sound_state_ext prog_tgt st_tgt)
-    (Hsim: state_lsim mrelT_ops prog_src prog_tgt ps_src ps_tgt pmrel mrel i st_src st_tgt)
+    height ps_src ps_tgt
+    emrel mrel
+    (Hp: match_stackframes height emrel ps_src ps_tgt)
+    (Hmrel_le: mrelT_ops.(le) emrel mrel)
+    (Hsim: state_lsim mrelT_ops prog_src prog_tgt ps_src ps_tgt emrel mrel i st_src st_tgt)
 .
+
+Lemma strong_nat_ind:
+  forall P : nat -> Prop,
+    (forall n : nat, (forall k : nat, (k < n -> P k)%nat) -> P n) ->
+    forall n : nat, P n.
+Proof.
+  intros P H.
+  assert (forall n, (forall k, k < n -> P k)%nat).
+  - induction n; intros k Hk.
+    + inversion Hk.
+    + apply Lt.le_lt_or_eq in Hk. destruct Hk as [Hk|Hk].
+      * apply Lt.lt_S_n in Hk. apply IHn. auto.
+      * inversion_clear Hk. apply H. apply IHn.
+  - intros. eapply H0. eauto.
+Qed.
 
 Lemma program_sim_forward_simulation:
   forward_simulation (semantics prog_src) (semantics prog_tgt).
@@ -79,11 +90,107 @@ Proof.
             (semantics prog_tgt)
             WF.wf
             match_states).
-  { admit. (* initial *)
+  { (* initial *)
+    intros. inversion H. 
+    exploit funct_ptr_translated; eauto. intros [tf [A B]].
+    exists WF.elt. exists (Callstate nil tf nil m0); split.
+    - econstructor; eauto.
+      eapply program_sim_init_mem_match; eauto.
+      replace (prog_main prog_tgt) with (prog_main prog_src).
+      erewrite symbols_preserved; eauto; auto.
+      destruct Hsim as [_ Hmain]. auto.
+      rewrite <- H3. inv B. inv Hsig.
+      destruct f, tf; auto.
+    - econstructor.
+      + apply match_stackframes_nil.
+      + instantiate (1 := mrel_init).
+        admit. (* le's reflexivity (spec) *)
+      + exploit funct_ptr_translated'; eauto.
+        intros [tf' [Htf' Hfundef_sim]]. rewrite A in Htf'. symmetry in Htf'. inv Htf'.
+        inv Hfundef_sim; destruct f, tf; inv Hsrc; inv Htgt.
+        { exploit Hsim0; try reflexivity. unfold F_future_sim. intros.
+          destruct H4 as [Hfunction_sim Hfunction_sig].
+          exploit Hfunction_sim.
+          { eapply program_sim_aux_le; eauto. }
+          intro X. inv X. eapply Hlsim; eauto.
+          { instantiate (1 := mrel_init).
+            admit. (* le's reflexivity (spec) *)
+          }
+          { admit. (* mrel_init satisfies m0 m0 (spec) *) }
+          { constructor. }
+          { apply sound_initial. auto. }
+          { apply sound_initial.
+            admit. (* initial_state (hard) *)
+          }
+        }
+        { admit. (* if external function is main? (hard) *)
+        }
   }
-  { admit. (* final *)
+  { (* final *)
+    simpl. intros. inv H0. inv H. punfold Hsim0. inv Hsim0.
+    - inv Hst_src.
+      revert height emrel Hmrel_le Hmrel_le_public Hp.
+      refine (strong_nat_ind _ _). intros height IHheight emrel Hmrel_le Hmrel_le_public Hp.
+      inversion Hp; symmetry in H0; subst.
+      { admit. (* sem_value (Vint r) ?b implies b = Vint r (spec) *)
+      }
+      { exploit Hreturn; eauto. instantiate (1 := WF.elt). intro Hsim'.
+        punfold Hsim'. inv Hsim'.
+        { inv Hst_src. inv Hst_tgt.
+          assert (Hle: mrelT_ops.(le) emrel0 mrel).
+          { admit. (* le's transitivity (spec) *) }
+          eauto.
+        }
+        { exfalso. eapply Hnfinal. constructor. }
+      }
+    - exfalso. eapply Hnfinal. constructor.
   }
-  { admit. (* step *)
+  { (* progress & preservation *)
+    intros. inv H0.
+    revert height i s2 ps_src ps_tgt emrel mrel Hp Hmrel_le Hsim0.
+    refine (strong_nat_ind _ _). intros height IHheight. intros.
+    punfold Hsim0. inv Hsim0.
+    { (* return *)
+      inversion Hp; symmetry in H1; subst; inv H.
+      assert (Hmrel_le': mrelT_ops.(le) emrel0 mrel).
+      { admit. (* le's transitivity (spec) *) }
+      exploit Hreturn; eauto.
+    }
+    { (* step *)
+      exploit Hpreserve; eauto. intros [i2 [st2_tgt [mrel2 [Hstep2 [Hle2 [Hmrel2 Hsim2]]]]]].
+      assert (Hmrel2_le: mrelT_ops.(le) emrel mrel2).
+      { admit. (* le's transitivity (spec) *) }
+      exists i2. exists st2_tgt. split; auto.
+      inv Hsim2.
+      { pclearbot. econstructor; eauto. }
+      { econstructor.
+        { eapply match_stackframes_cons; eauto.
+          instantiate (1 := stack_tgt). instantiate (1 := stack_src). intros. subst.
+          exploit Hreturn; eauto. intro Hsim2. pclearbot. eauto.
+        }
+        { instantiate (1 := mrel2). admit. (* le's reflexivity (spec) *) }
+        { inv Hfundef. exploit funct_ptr_translated'; eauto.
+          intros [tf [Htf Hfundef_sim]]. unfold Genv.find_funct_ptr in Htf.
+          unfold fundef in *. rewrite Htgt in Htf. symmetry in Htf. inv Htf.
+          inv Hfundef_sim; destruct fundef_src, fundef_tgt; inv Hsrc0; inv Htgt0.
+          { exploit Hsim0; try reflexivity. unfold F_future_sim. intros.
+            destruct H0 as [Hfunction_sim Hfunction_sig].
+            exploit Hfunction_sim.
+            { eapply program_sim_aux_le; eauto. }
+            intro X. inv X. eapply Hlsim; eauto.
+            { eapply sound_past_step; eauto. }
+            { admit. (* sound_past_step for Plus|Star (easy) *) }
+          }
+          { pfold. constructor.
+            { intros ? Hfinal. inv Hfinal. }
+            { eapply sound_past_step; eauto. }
+            { admit. (* sound_past_step for Plus|Star (easy) *) }
+            intros. exists WF.elt.
+            admit. (* external function (hard) *)
+          }
+        }
+      }
+    }
   }
   { eapply symbols_preserved; eauto. }
 Qed.
